Started work on annotated system

theories/Core/Syntactic/SystemAnnotated/Definitions.v
@@ -1,150 +1,196 @@
+From Coq Require Import String.
 From McPTS Require Import PtsSignature.
 From McPTS.Core Require Import Base.
 From McPTS.Core.Syntactic Require Export Syntax System.
 Import Syntax_Notations.
 
-Reserved Notation "⊫ Γ 'with' anns" (in custom judg at level 80, Γ custom exp, anns constr).
-Reserved Notation "Γ 'with' anns ⊫ M : A @ s" (in custom judg at level 80, Γ custom exp, anns constr, M custom exp, A custom exp, s custom exp).
-Reserved Notation "Γ 'with' anns ⊫ A @ s" (in custom judg at level 80, Γ custom exp, anns constr, A custom exp, s custom exp).
-Reserved Notation "Γ 'with' anns ⊫s σ : Δ 'with' anns'" (in custom judg at level 80, Γ custom exp, anns constr, σ custom exp, Δ custom exp, anns' constr).
-Reserved Notation "'#' x : A '@' so ∈ Γ 'with' anns" (in custom judg at level 80, x constr at level 0, so constr, anns constr, A custom exp, Γ custom exp at level 50).
-Notation ctx_anns := (fun (P : PtsSig) => list (SortOption P)%type).
+(** * Notation for annotated judgments *)
 
+(** ** Context lookups *)
+Reserved Notation "'`#' x : A @ so ∈ Δ @ annsΔ" (in custom judg at level 80, x constr at level 0, A custom exp, so constr, Δ custom exp, annsΔ custom exp).
+Reserved Notation "'#' x : A '@' so ∈ Γ @ annsΓ" (in custom judg at level 80, x constr at level 0, A custom exp, so constr, Γ custom exp, annsΓ custom exp).
+(** ** Well-formed contexts *)
+Reserved Notation "⊫ Δ @ annsΔ" (in custom judg at level 80, Δ custom exp, annsΔ custom exp).
+Reserved Notation "Δ @ annsΔ ⊫ Γ @ annsΓ" (in custom judg at level 80, Δ custom exp, annsΔ custom exp, Γ custom exp, annsΓ custom exp).
+(** ** Well-formed expressions *)
+Reserved Notation "Δ @ annsΔ ; Γ @ annsΓ ⊫ M : A @ so" (in custom judg at level 80, Δ custom exp, annsΔ custom exp, Γ custom exp, annsΓ custom exp, M custom exp, A custom exp, so custom exp).
+(** ** Well-formed types *)
+Reserved Notation "Δ @ annsΔ ; Γ @ annsΓ ⊫ A @ so" (in custom judg at level 80, Δ custom exp, annsΔ custom exp, Γ custom exp, annsΓ custom exp, A custom exp, so custom exp).
+(** ** Well-formed substitutions *)
+Reserved Notation "Δ @ annsΔ ; Γ @ annsΓ ⊫s σ : Γ' @ annsΓ'" (in custom judg at level 80, Δ custom exp, annsΔ custom exp, Γ custom exp, annsΓ custom exp, σ custom exp, Γ' custom exp, annsΓ' custom exp).
+
+(** ** Shorthands for annotations *)
+Notation gctx_anns := (fun (P : PtsSig) => list (SortOption P)%type).
+Notation ctx_anns := (fun (P : PtsSig) => list (SortOption P)%type).
+Notation typ_ann := (fun (P : PtsSig) => SortOption P).
+  
 Generalizable All Variables.
 
-Inductive anns_lookup {P : PtsSig} : nat -> typ P -> SortOption P -> ctx_anns P -> ctx P -> Prop :=
-| here : `( {{ #0 : A[Wk] @ so ∈ Γ,A with (so::anns) }})
-| there : `( {{ #n : A @ so ∈ Γ with anns }} -> {{ #(S n) : A[Wk] @ so ∈ Γ, B with (so'::anns) }} )
-where "'#' x : A '@' so ∈ Γ 'with' anns" := (anns_lookup x A so anns Γ) (in custom judg).
+(** * Definitions of annotated judgments *)
+(** Lookup in global contexts *)
+Inductive gctx_lookup_ann {P : PtsSig} : string -> typ P -> typ_ann P -> gctx P -> gctx_anns P -> Prop :=
+| ghere_ann : `( {{ `#x : A @ so ∈ Δ, x:A @ annsΔ, so }} )
+| gthere_ann : `( {{ `#x : A @ so ∈ Δ @ annsΔ }} ->
+                  x <> y ->
+                  {{ `#x : A @so ∈ Δ, y:B @ annsΔ, so' }} )
+where "'`#' x : A @ so ∈ Δ @ annsΔ" := (gctx_lookup_ann x A so Δ annsΔ) (in custom judg).
 
 #[export]
-Hint Constructors anns_lookup : mcpts.
+Hint Constructors gctx_lookup_ann : mcpts.
+ 
+(** Lokup in local contexts *)
+Inductive ctx_lookup_ann {P : PtsSig} : nat -> typ P -> typ_ann P -> ctx P -> ctx_anns P -> Prop :=
+| here_ann : `( {{ #0 : A[Wk] @ so ∈ Γ,A @ annsΓ, so }})
+| there_ann : `( {{ #n : A @ so ∈ Γ @ annsΓ }} -> {{ #(S n) : A[Wk] @ so ∈ Γ, B @ annsΓ, so' }} )
+where "'#' x : A '@' so ∈ Γ @ annsΓ" := (ctx_lookup_ann x A so Γ annsΓ) (in custom judg).
 
-Inductive wf_ctx_ann {P} : ctx_anns P -> ctx P -> Prop :=
-| wfa_ctx_empty : {{ ⊫ ⋅ with nil}}
+#[export]
+Hint Constructors ctx_lookup_ann : mcpts.
+
+Inductive wf_gctx_ann {P : PtsSig} : gctx P -> gctx_anns P -> Prop :=
+| wf_gctx_empty_ann : {{ ⊫ ⋅ @ ⋅ }}
+| wf_gctx_extend_ann :
+  `( {{ ⊫ Δ @ annsΔ }} ->
+     {{ Δ @ annsΔ ; ⋅ @ ⋅ ⊫ A @ so }} ->
+     {{ `#x ∉ Δ }} ->
+     {{ ⊫ Δ, x:A @ annsΔ , so }} )
+where "⊫ Δ @ annsΔ" := (wf_gctx_ann Δ annsΔ) (in custom judg)
+
+with wf_ctx_ann {P : PtsSig} : gctx P -> gctx_anns P -> ctx P -> ctx_anns P -> Prop :=
+| wfa_ctx_empty :
+  `( {{ ⊫ Δ @ annsΔ }} ->
+     {{ Δ @ annsΔ ⊫ ⋅ @ ⋅ }} )
 | wfa_ctx_enxtend :
-  `( {{ ⊫ Γ with anns }} ->
-     {{ Γ with anns ⊫ A @ so }} ->
-     {{ ⊫ Γ, A with so::anns }} )
-where "⊫ Γ 'with' anns" := (wf_ctx_ann anns Γ) (in custom judg) : type_scope
-with wf_exp_ann {P} : ctx_anns P -> ctx P -> typ P -> SortOption P -> exp P -> Prop :=
+  `( {{ Δ @ annsΔ ⊫ Γ @ annsΓ }} ->
+     {{ Δ @ annsΔ ; Γ @ annsΓ ⊫ A @ so }} ->
+     {{ Δ @ annsΔ ⊫ Γ, A @ annsΓ, so }} )
+where "Δ @ annsΔ ⊫ Γ @ annsΓ" := (wf_ctx_ann Δ annsΔ Γ annsΓ) (in custom judg) : type_scope
+
+with wf_exp_ann {P : PtsSig} : gctx P -> gctx_anns P -> ctx P -> ctx_anns P -> typ P -> typ_ann P -> exp P -> Prop :=
 (** Sorts *)
-| wfa_st :
+| wf_exp_st_ann :
   `( Ax_typ P s1 s2 ->
-     {{ ⊫ Γ with anns }} ->
-     {{ Γ with anns ⊫ Sort@s1 : Sort@s2 @ ^so_None }} )
+     {{ Δ @ annsΔ ⊫ Γ @ annsΓ }} ->
+     {{ Δ @ annsΔ ; Γ @ annsΓ ⊫ Sort@s1 : Sort@s2 @ ^so_None }} )
 
 (** Functions *)
-| wfa_pi :
+| wf_exp_pi_ann :
   `( forall (r : Ru_pi P s1 s2 s3),
-        {{ Γ with anns ⊫ A : Sort@s1 @ so1 }} ->
-        {{ Γ, A with (so_Some s1)::anns ⊫ B : Sort@s2 @ so2 }} ->
-        {{ Γ with anns ⊫ Π r A B : Sort@s3 @ ^so_None }} )
-| wfa_fn :
+        {{ Δ @ annsΔ ; Γ @ annsΓ ⊫ A : Sort@s1 @ so1 }} ->
+        {{ Δ @ annsΔ ; Γ, A @ annsΓ, ^(so_Some s1) ⊫ B : Sort@s2 @ so2 }} ->
+        {{ Δ @ annsΔ ; Γ @ annsΓ ⊫ Π r A B : Sort@s3 @ ^so_None }} )
+| wf_exp_fn_ann :
   `( forall (r : Ru_pi P s1 s2 s3),
-        {{ Γ with anns ⊫ A : Sort@s1 @ so1 }} ->
-        {{ Γ, A with (so_Some s1)::anns ⊫ B : Sort@s2 @ so2 }} ->
-        {{ Γ, A with (so_Some s1)::anns ⊫ M : B @ ^(so_Some s2) }} ->
-        {{ Γ with anns ⊫ λ r A B M : Π r A B @ ^(so_Some s3) }} )
-| wfa_app :
+        {{ Δ @ annsΔ ; Γ @ annsΓ ⊫ A : Sort@s1 @ so1 }} ->
+        {{ Δ @ annsΔ ; Γ, A @ annsΓ, ^(so_Some s1) ⊫ B : Sort@s2 @ so2 }} ->
+        {{ Δ @ annsΔ ; Γ, A @ annsΓ, ^(so_Some s1) ⊫ M : B @ ^(so_Some s2) }} ->
+        {{ Δ @ annsΔ ; Γ @ annsΓ ⊫ λ r A B M : Π r A B @ ^(so_Some s3) }} )
+| wf_exp_app_ann :
   `( forall (r : Ru_pi P s1 s2 s3),
-        {{ Γ with anns ⊫ A : Sort@s1 @ so1 }} ->
-        {{ Γ, A with (so_Some s1)::anns ⊫ B : Sort@s2 @ so2 }} ->
-        {{ Γ with anns ⊫ M : Π r A B @ ^(so_Some s3) }} ->
-        {{ Γ with anns ⊫ N : A @ ^(so_Some s1) }} ->
-        {{ Γ with anns ⊫ M N : B[Id,,N] @ ^(so_Some s2) }} )
+        {{ Δ @ annsΔ ; Γ @ annsΓ ⊫ A : Sort@s1 @ so1 }} ->
+        {{ Δ @ annsΔ ; Γ, A @ annsΓ, ^(so_Some s1) ⊫ B : Sort@s2 @ so2 }} ->
+        {{ Δ @ annsΔ ; Γ @ annsΓ ⊫ M : Π r A B @ ^(so_Some s3) }} ->
+        {{ Δ @ annsΔ ; Γ @ annsΓ ⊫ N : A @ ^(so_Some s1) }} ->
+        {{ Δ @ annsΔ ; Γ @ annsΓ ⊫ M N : B[Id,,N] @ ^(so_Some s2) }} )
 
 (** Variables *)
-| wfa_vlookup :
-  `( {{ ⊫ Γ with anns }} ->
-     {{ #x : A@so ∈ Γ with anns }} ->
-     {{ Γ with anns ⊫ #x : A @ so }} )
-
+| wf_exp_vlookup_ann :
+  `( {{ Δ @ annsΔ ⊫ Γ @ annsΓ }} ->
+     {{ #x : A@so ∈ Γ @ annsΓ }} ->
+     {{ Δ @ annsΔ ; Γ @ annsΓ ⊫ #x : A @ so }} )
+| wf_exp_gvlookup_ann :
+  `( {{ Δ @ annsΔ ; Γ @ annsΓ ⊫s σ : ⋅ @ ⋅ }} ->
+     {{ `#x : A @ so ∈ Δ @ annsΔ }} ->
+     {{ Δ @ annsΔ ; Γ @ annsΓ ⊫ `#x : A[σ] @ so }} )
+   
 (** Naturals *)
-| wfa_nat :
+| wf_exp_nat_ann :
   `( forall (r : Ru_nat P sn),
-        {{ ⊫ Γ with anns}} ->
-        {{ Γ with anns ⊫ ℕ : Sort@sn @ ^so_None }} )
-| wfa_zero :
+        {{ Δ @ annsΔ ⊫ Γ @ annsΓ}} ->
+        {{ Δ @ annsΔ ; Γ @ annsΓ ⊫ ℕ : Sort@sn @ ^so_None }} )
+| wf_exp_zero_ann :
   `( forall (r : Ru_nat P sn),
-        {{ ⊫ Γ with anns }} ->
-        {{ Γ with anns ⊫ zero : ℕ @ ^(so_Some sn) }} )
-| wfa_succ :
+        {{ Δ @ annsΔ ⊫ Γ @ annsΓ }} ->
+        {{ Δ @ annsΔ ; Γ @ annsΓ ⊫ zero : ℕ @ ^(so_Some sn) }} )
+| wf_exp_succ_ann :
   `( forall (r : Ru_nat P sn),
-        {{ Γ with anns ⊫ M : ℕ @ ^(so_Some sn) }} ->
-        {{ Γ with anns ⊫ succ M : ℕ @ ^(so_Some sn) }} )
-| wfa_rec :
+        {{ Δ @ annsΔ ; Γ @ annsΓ ⊫ M : ℕ @ ^(so_Some sn) }} ->
+        {{ Δ @ annsΔ ; Γ @ annsΓ ⊫ succ M : ℕ @ ^(so_Some sn) }} )
+| wf_exp_rec_ann :
   `( forall (r : Ru_nat P sn),
-        {{ Γ, ℕ with (so_Some sn)::anns ⊫ A @ so }} ->
-        {{ Γ with anns ⊫ MZ : A[Id,,zero] @ so }} ->
-        {{ Γ, ℕ, A with so ::(so_Some sn)::anns ⊫ MS : A[Wk∘Wk,,succ #1] @ so  }} ->
-        {{ Γ with anns ⊫ M : ℕ @ ^(so_Some sn) }} ->
-        {{ Γ with anns ⊫ rec M return A | zero -> MZ | succ -> MS end : A[Id,,M] @ so }} )
+        {{ Δ @ annsΔ ; Γ, ℕ @ annsΓ, ^(so_Some sn) ⊫ A @ so }} ->
+        {{ Δ @ annsΔ ; Γ @ annsΓ ⊫ MZ : A[Id,,zero] @ so }} ->
+        {{ Δ @ annsΔ ; Γ, ℕ, A @ annsΓ, ^(so_Some sn), so ⊫ MS : A[Wk∘Wk,,succ #1] @ so  }} ->
+        {{ Δ @ annsΔ ; Γ @ annsΓ ⊫ M : ℕ @ ^(so_Some sn) }} ->
+        {{ Δ @ annsΔ ; Γ @ annsΓ ⊫ rec M return A | zero -> MZ | succ -> MS end : A[Id,,M] @ so }} )
 
 (** explicit substitutions *)
-| wfa_exp_sub:
-  `( {{ Γ with anns ⊫s σ : Δ with anns' }} ->
-     {{ Δ with anns' ⊫ M : A @ so }} ->
-     {{ Δ with anns' ⊫ A @ so }} ->
-     {{ Γ with anns ⊫ M[σ] : A[σ] @ so }} )
+| wf_exp_sub_ann:
+  `( {{ Δ @ annsΔ ; Γ @ annsΓ ⊫s σ : Γ' @ annsΓ' }} ->
+     {{ Δ @ annsΔ ; Γ' @ annsΓ' ⊫ M : A @ so }} ->
+     {{ Δ @ annsΔ ; Γ' @ annsΓ' ⊫ A @ so }} ->
+     {{ Δ @ annsΔ ; Γ @ annsΓ ⊫ M[σ] : A[σ] @ so }} )
 
 (** Conversions *)
-| wfa_exp_conv :
-  `( {{ Γ with anns ⊫ M : A @ so }} ->
-     {{ Γ with anns ⊫ A' @ so' }} ->
-     {{ Γ ⊢ A ⊆ A' }} ->
-     {{ Γ with anns ⊫ M : A' @ so' }} )
-| wfa_exp_conv_ann :
-  `( {{ Γ with anns ⊫ M : A @ so }} ->
-     {{ Γ with anns ⊫ A @ so' }} ->
-     {{ Γ with anns ⊫ M : A @ so' }} )
-where "Γ 'with' anns ⊫ M : A @ so" := (wf_exp_ann anns Γ A so M) (in custom judg) : type_scope
+| wf_exp_conv_ann :
+  `( {{ Δ @ annsΔ ; Γ @ annsΓ ⊫ M : A @ so }} ->
+     {{ Δ @ annsΔ ; Γ @ annsΓ ⊫ A' @ so' }} ->
+     {{ Δ ; Γ ⊢ A ⊆ A' }} ->
+     {{ Δ @ annsΔ ; Γ @ annsΓ ⊫ M : A' @ so' }} )
+| wfa_exp_conv_annotation :
+  `( {{ Δ @ annsΔ ; Γ @ annsΓ ⊫ M : A @ so }} ->
+     {{ Δ @ annsΔ ; Γ @ annsΓ ⊫ A @ so' }} ->
+     {{ Δ @ annsΔ ; Γ @ annsΓ ⊫ M : A @ so' }} )
 
-with wf_typ_ann {P} : ctx_anns P -> ctx P -> typ P -> SortOption P -> Prop :=
-| wfa_typ_st :
-  `( {{ ⊫ Γ with anns }} ->
-     {{ Γ with anns ⊫ Sort@s @ ^so_None }} )
-| wfa_typ_exp :
-  `( {{ Γ with anns ⊫ A : Sort@s @ so }} ->
-     {{ Γ with anns ⊫ A @ ^(so_Some s) }} )
-| wfa_typ_sub :
-  `( {{ Γ with anns ⊫s σ : Δ with anns' }} ->
-     {{ Δ with anns' ⊫ A @ so}} ->
-     {{ Γ with anns ⊫ A[σ] @ so }} )
-where "Γ 'with' anns ⊫ A @ so" := (wf_typ_ann anns Γ A so) (in custom judg) : type_scope
-with wf_sub_ann {P} : ctx_anns P -> ctx_anns P -> ctx P -> ctx P -> sub P -> Prop :=
-| wfa_sub_id :
-  `( {{ ⊫ Γ with anns }} ->
-     {{ Γ with anns ⊫s Id : Γ with anns }} )
+where "Δ @ annsΔ ; Γ @ annsΓ ⊫ M : A @ so" := (wf_exp_ann Δ annsΔ Γ annsΓ A so M) (in custom judg)
+
+with wf_typ_ann {P : PtsSig} : gctx P -> gctx_anns P -> ctx P -> ctx_anns P -> typ P -> typ_ann P -> Prop :=
+| wf_typ_st_ann :
+  `( {{ Δ @ annsΔ ⊫ Γ @ annsΓ }} ->
+     {{ Δ @ annsΔ ; Γ @ annsΓ ⊫ Sort@s @ ^so_None }} )
+| wf_typ_exp_ann :
+  `( {{ Δ @ annsΔ ; Γ @ annsΓ ⊫ A : Sort@s @ so }} ->
+     {{ Δ @ annsΔ ; Γ @ annsΓ ⊫ A @ ^(so_Some s) }} )
+| wf_typ_sub_ann :
+  `( {{ Δ @ annsΔ ; Γ @ annsΓ ⊫s σ : Γ' @ annsΓ' }} ->
+     {{ Δ @ annsΔ ; Γ' @ annsΓ' ⊫ A @ so}} ->
+     {{ Δ @ annsΔ ; Γ @ annsΓ ⊫ A[σ] @ so }} )
+where "Δ @ annsΔ ; Γ @ annsΓ ⊫ A @ so" := (wf_typ_ann Δ annsΔ Γ annsΓ A so) (in custom judg)
+
+with wf_sub_ann {P : PtsSig} : gctx P -> gctx_anns P -> ctx P -> ctx_anns P -> ctx P -> ctx_anns P -> sub P -> Prop :=
+| wf_sub_id_ann :
+  `( {{ Δ @ annsΔ ⊫ Γ @ annsΓ }} ->
+     {{ Δ @ annsΔ ; Γ @ annsΓ ⊫s Id : Γ @ annsΓ }} )
 | wfa_sub_weaken :
-  `( {{ ⊫ Γ, A with so::anns }} ->
-     {{ Γ, A with so::anns ⊫s Wk : Γ with anns}} )
+  `( {{ Δ @ annsΔ ⊫ Γ, A @ annsΓ, so }} ->
+     {{ Δ @ annsΔ ; Γ, A @ annsΓ, so ⊫s Wk : Γ @ annsΓ }} )
 | wfa_sub_compose :
-  `( {{ Γ1 with anns1 ⊫s σ2 : Γ2 with anns2 }} ->
-     {{ Γ2 with anns2 ⊫s σ1 : Γ3 with anns3 }} ->
-     {{ Γ1 with anns1 ⊫s σ1∘σ2 : Γ3 with anns3 }} )
+  `( {{ Δ @ annsΔ ; Γ1 @ annsΓ1 ⊫s σ2 : Γ2 @ annsΓ2 }} ->
+     {{ Δ @ annsΔ ; Γ2 @ annsΓ2 ⊫s σ1 : Γ3 @ annsΓ3 }} ->
+     {{ Δ @ annsΔ ; Γ1 @ annsΓ1 ⊫s σ1∘σ2 : Γ3 @ annsΓ3 }} )
 | wfa_sub_extend :
-  `( {{ Γ with anns ⊫s σ : Δ with anns' }} ->
-     {{ Δ with anns' ⊫ A @ so }} ->
-     {{ Γ with anns ⊫ M : A[σ] @ so }} ->
-     {{ Γ with anns ⊫s σ,,M : Δ, A with so::anns'  }} )
+  `( {{ Δ @ annsΔ ; Γ @ annsΓ ⊫s σ : Γ' @ annsΓ' }} ->
+     {{ Δ @ annsΔ ; Γ' @ annsΓ' ⊫ A @ so }} ->
+     {{ Δ @ annsΔ ; Γ @ annsΓ ⊫ M : A[σ] @ so }} ->
+     {{ Δ @ annsΔ ; Γ @ annsΓ ⊫s σ,,M : Γ', A @ annsΓ', so  }} )
 | wfa_sub_conv :
-  `( {{ Γ with anns ⊫s σ : Δ with anns' }} ->
-     {{ ⊫ Δ' with anns'' }} ->
-     {{ ⊢ Δ ⊆ Δ' }} ->
-     {{ Γ with anns ⊫s σ : Δ' with anns'' }} )
-where "Γ 'with' anns ⊫s σ : Δ 'with' anns'" := (wf_sub_ann anns anns' Γ Δ σ) (in custom judg) : type_scope.
-
+  `( {{ Δ @ annsΔ ; Γ @ annsΓ ⊫s σ : Γ' @ annsΓ' }} ->
+     {{ Δ @ annsΔ ⊫ Γ'' @ annsΓ'' }} ->
+     {{ Δ ⊢ Γ' ⊆ Γ'' }} ->
+     {{ Δ @ annsΔ ; Γ @ annsΓ ⊫s σ : Γ'' @ annsΓ'' }} )
+where "Δ @ annsΔ ; Γ @ annsΓ ⊫s σ : Γ' @ annsΓ'" := (wf_sub_ann Δ annsΔ Γ annsΓ Γ' annsΓ' σ) (in custom judg).
 
 #[export]
-Hint Constructors wf_ctx_ann wf_exp_ann wf_typ_ann wf_sub_ann : mcpts.
+Hint Constructors wf_gctx_ann wf_ctx_ann wf_exp_ann wf_typ_ann wf_sub_ann : mcpts.
 
 
-Scheme wf_ctx_ann_mut_ind := Induction for wf_ctx_ann Sort Prop
-with  wf_exp_ann_mut_ind := Induction for wf_exp_ann Sort Prop
+Scheme wf_gctx_ann_mut_ind := Induction for wf_gctx_ann Sort Prop
+with wf_ctx_ann_mut_ind := Induction for wf_ctx_ann Sort Prop
+with wf_exp_ann_mut_ind := Induction for wf_exp_ann Sort Prop
 with wf_typ_ann_mut_ind := Induction for wf_typ_ann Sort Prop
 with wf_sub_ann_mut_ind := Induction for wf_sub_ann Sort Prop.
 Combined Scheme syntactic_wf_ann_mut_ind from
+  wf_gctx_ann_mut_ind,
   wf_ctx_ann_mut_ind,
   wf_exp_ann_mut_ind,
   wf_typ_ann_mut_ind,
