theories/Core/Syntactic/SystemAnnotated/Lemmas.v
@@ -4,9 +4,316 @@ From McPTS.Core.Syntactic Require Import Syntax System Corollaries.
 From McPTS.Core.Syntactic.SystemAnnotated Require Import Definitions.
 Import Syntax_Notations.
 
+(** * Basic properties of annotated judgments *)
+
+(** ** Inversion for global contexts *)
+Lemma wf_gctx_ann_decomp {P : PtsSig} : forall {Δ : gctx P} {annsΔ A so x},
+    {{ ⊫ Δ, x:A @ annsΔ, so }} -> {{ ⊫ Δ @ annsΔ }} /\ {{ Δ @ annsΔ ; ⋅ @ ⋅ ⊫ A @ so }}.
+Proof with now eauto.
+  inversion 1...
+Qed.
+
+Lemma wf_gctx_ann_decomp_left {P : PtsSig} : forall {Δ : gctx P} {annsΔ A so x},
+    {{ ⊫ Δ, x:A @ annsΔ, so }} -> {{ ⊫ Δ @ annsΔ }}.
+Proof with easy.
+  intros * ?%wf_gctx_ann_decomp...
+Qed.
+
+Lemma wf_gctx_ann_decomp_right {P : PtsSig} : forall {Δ : gctx P} {annsΔ A so x},
+    {{ ⊫ Δ, x:A @ annsΔ, so }} -> {{ Δ @ annsΔ ; ⋅ @ ⋅ ⊫ A @ so }}.
+Proof with easy.
+  intros * ?%wf_gctx_ann_decomp...
+Qed.
 
 #[local]
-Ltac gen_annotated_judg_IH P ann_ctx ann_exp ann_typ ann_sub :=
+Hint Resolve wf_gctx_ann_decomp wf_gctx_ann_decomp_left wf_gctx_ann_decomp_right : mcpts.
+
+(** ** Inversion for local contexts *)
+Lemma wf_ctx_ann_decomp {P : PtsSig} : forall {Δ : gctx P} {annsΔ Γ annsΓ A so},
+    {{ Δ @ annsΔ ⊫ Γ, A @ annsΓ, so }} -> {{ Δ @ annsΔ ⊫ Γ @ annsΓ }} /\ {{ Δ @ annsΔ ; Γ @ annsΓ ⊫ A @ so }}.
+Proof with now eauto.
+  inversion 1...
+Qed.
+
+Lemma wf_ctx_ann_decomp_left {P : PtsSig} : forall {Δ : gctx P} {annsΔ Γ annsΓ A so},
+    {{ Δ @ annsΔ ⊫ Γ, A @ annsΓ, so }} -> {{ Δ @ annsΔ ⊫ Γ @ annsΓ }}.
+Proof with easy.
+  intros * ?%wf_ctx_ann_decomp...
+Qed.
+
+Lemma wf_ctx_ann_decomp_right {P : PtsSig} : forall {Δ : gctx P} {annsΔ Γ annsΓ A so},
+    {{ Δ @ annsΔ ⊫ Γ, A @ annsΓ, so }} -> {{ Δ @ annsΔ ; Γ @ annsΓ ⊫ A @ so }}.
+Proof with easy.
+  intros * ?%wf_ctx_ann_decomp...
+Qed.
+
+#[local]
+Hint Resolve wf_ctx_ann_decomp wf_ctx_ann_decomp_left wf_ctx_ann_decomp_right : mcpts.
+
+(** ** Basic context presupposition *)
+(** For local contexts *)
+Lemma presup_wf_ctx_ann {P : PtsSig} : forall {Δ : gctx P} {annsΔ Γ annsΓ},
+    {{ Δ @ annsΔ ⊫ Γ @ annsΓ }} -> {{ ⊫ Δ @ annsΔ }}.
+Proof.
+  induction 1; mauto 2.
+Qed.
+
+#[local]
+Hint Resolve presup_wf_ctx_ann : mcpts.
+
+(** For well-formed substitutions *)
+Lemma presup_wf_sub_ann {P : PtsSig} : forall {Δ : gctx P} {annsΔ Γ annsΓ Γ' annsΓ' σ},
+    {{ Δ @ annsΔ ; Γ @ annsΓ ⊫s σ : Γ' @ annsΓ' }} -> {{ ⊫ Δ @ annsΔ }} /\ {{ Δ @ annsΔ ⊫ Γ @ annsΓ }} /\ {{ Δ @ annsΔ ⊫ Γ' @ annsΓ' }}.
+Proof.
+  induction 1; destruct_pairs; repeat split; mauto 2.
+Qed.
+
+Lemma presup_wf_sub_ann_gctx {P : PtsSig} : forall {Δ : gctx P} {annsΔ Γ annsΓ Γ' annsΓ' σ},
+    {{ Δ @ annsΔ ; Γ @ annsΓ ⊫s σ : Γ' @ annsΓ' }} -> {{ ⊫ Δ @ annsΔ }}.
+Proof with easy.
+  intros * ?%presup_wf_sub_ann...
+Qed.
+
+Lemma presup_wf_sub_ann_left {P : PtsSig} : forall {Δ : gctx P} {annsΔ Γ annsΓ Γ' annsΓ' σ},
+    {{ Δ @ annsΔ ; Γ @ annsΓ ⊫s σ : Γ' @ annsΓ' }} -> {{ Δ @ annsΔ ⊫ Γ @ annsΓ }}.
+Proof with easy.
+  intros * ?%presup_wf_sub_ann...
+Qed.
+
+Lemma presup_wf_sub_ann_right {P : PtsSig} : forall {Δ : gctx P} {annsΔ Γ annsΓ Γ' annsΓ' σ},
+    {{ Δ @ annsΔ ; Γ @ annsΓ ⊫s σ : Γ' @ annsΓ' }} -> {{ Δ @ annsΔ ⊫ Γ' @ annsΓ' }}.
+Proof with easy.
+  intros * ?%presup_wf_sub_ann...
+Qed.
+
+#[local]
+Hint Resolve presup_wf_sub_ann presup_wf_sub_ann_gctx presup_wf_sub_ann_left presup_wf_sub_ann_right : mcpts.
+
+(** For well-formed expressions *)
+Lemma presup_wf_exp_ann {P : PtsSig} : forall {Δ : gctx P} {annsΔ Γ annsΓ A so M},
+    {{ Δ @ annsΔ ; Γ @ annsΓ ⊫ M : A @ so }} -> {{ ⊫ Δ @ annsΔ }} /\ {{ Δ @ annsΔ ⊫ Γ @ annsΓ }}.
+Proof.
+  induction 1; destruct_pairs; split; mauto 2.
+Qed.  
+
+Lemma presup_wf_exp_ann_gctx {P : PtsSig} : forall {Δ : gctx P} {annsΔ Γ annsΓ A so M},
+    {{ Δ @ annsΔ ; Γ @ annsΓ ⊫ M : A @ so }} -> {{ ⊫ Δ @ annsΔ }}.
+Proof with easy.
+  intros * ?%presup_wf_exp_ann...
+Qed.
+
+Lemma presup_wf_exp_ann_ctx {P : PtsSig} : forall {Δ : gctx P} {annsΔ Γ annsΓ A so M},
+    {{ Δ @ annsΔ ; Γ @ annsΓ ⊫ M : A @ so }} -> {{ Δ @ annsΔ ⊫ Γ @ annsΓ }}.
+Proof with easy.
+  intros * ?%presup_wf_exp_ann...
+Qed.
+
+#[local]
+Hint Resolve presup_wf_exp_ann presup_wf_exp_ann_gctx presup_wf_exp_ann_ctx : mcpts.
+
+(** For well-formed types *)
+Lemma presup_wf_typ_ann {P : PtsSig} : forall {Δ : gctx P} {annsΔ Γ annsΓ A so},
+    {{ Δ @ annsΔ ; Γ @ annsΓ ⊫ A @ so }} -> {{ ⊫ Δ @ annsΔ }} /\ {{ Δ @ annsΔ ⊫ Γ @ annsΓ }}.
+Proof.
+  induction 1; destruct_pairs; split; mauto 2.
+Qed.  
+
+Lemma presup_wf_typ_ann_gctx {P : PtsSig} : forall {Δ : gctx P} {annsΔ Γ annsΓ A so},
+    {{ Δ @ annsΔ ; Γ @ annsΓ ⊫ A @ so }} -> {{ ⊫ Δ @ annsΔ }}.
+Proof with easy.
+  intros * ?%presup_wf_typ_ann...
+Qed.
+
+Lemma presup_wf_typ_ann_ctx {P : PtsSig} : forall {Δ : gctx P} {annsΔ Γ annsΓ A so },
+    {{ Δ @ annsΔ ; Γ @ annsΓ ⊫ A @ so }} -> {{ Δ @ annsΔ ⊫ Γ @ annsΓ }}.
+Proof with easy.
+  intros * ?%presup_wf_typ_ann...
+Qed.
+
+#[local]
+Hint Resolve presup_wf_typ_ann presup_wf_typ_ann_gctx presup_wf_typ_ann_ctx : mcpts.
+
+(** ** Useful tactics related to presupposition *)
+#[local]
+Ltac invert_wf_gctx_ann1 H :=
+  match type of H with
+  | {{ ⊫ ^?Δ, ^?x : ^?A @ ^?annsΔ, ^?so }} =>
+      let HΔ := fresh "HΔ" in
+      let HA := fresh "HA" in
+      let Hx := fresh "Hx" in
+      pose proof wf_gctx_ann_decomp H as [HΔ [HA Hx]];
+      match goal with
+      | _: {{ Δ @ annsΔ ; ⋅ @ ⋅ ⊫ A @ so }} |- _ => clear HA
+      | _: __mark__ _ {{ Δ @ annsΔ ; ⋅ @ ⋅ ⊫ A @ so }} |- _ => clear HA
+      end
+  end.
+
+#[local]
+Ltac invert_wf_gctx_ann :=
+  (on_all_hyp: fun H => invert_wf_gctx_ann1 H);
+  clear_dups.
+
+#[local]
+Ltac invert_wf_ctx_ann1 H :=
+  match type of H with
+  | {{ ^?Δ @ ^?annsΔ ⊫ ^?Γ, ^?A @ ^?annsΓ, ^?so }} =>
+      let HΓ := fresh "HΓ" in
+      let HA := fresh "HA" in
+      pose proof wf_ctx_ann_decomp H as [HΓ HA];
+      match goal with
+      | _: {{ Δ ; Γ ⊢ A }} |- _ => clear HA
+      | _: __mark__ _ {{ Δ ; Γ ⊢ A }} |- _ => clear HA
+      end
+  end.
+
+Ltac invert_wf_ctx_ann :=
+  (on_all_hyp: fun H => invert_wf_ctx_ann1 H);
+  clear_dups.
+
+#[local]
+Ltac gen_presup_ann H :=
+  match type of H with
+  | {{ ^?Δ @ ^?annsΔ ⊫ ^?Γ @ ^?annsΓ }} =>
+      let HΔ := fresh "HΔ" in
+      pose proof presup_wf_ctx_ann H as HΔ
+  | {{ ^?Δ @ ^?annsΔ ; ^?Γ @ ^?annsΓ ⊫ ^?M : ^?A @ ^?so }} =>
+      let HΔ := fresh "HΔ" in
+      let HΓ := fresh "HΓ" in
+      pose proof presup_wf_exp_ann H as [HΔ HΓ]
+  | {{ ^?Δ @ ^?annsΔ ; ^?Γ @ ^?annsΓ ⊫ ^?A @ ^?so }} =>
+      let HΔ := fresh "HΔ" in
+      let HΓ := fresh "HΓ" in
+      pose proof presup_wf_typ_ann H as [HΔ HΓ]
+  | {{ ^?Δ @ ^?annsΔ ; ^?Γ @ ^?annsΓ ⊫s ^?σ : ^?Γ' @ ^?annsΓ' }} =>
+      let HΔ := fresh "HΔ" in
+      let HΓ := fresh "HΓ" in
+      let HΓ' := fresh "HΓ'" in
+      pose proof presup_wf_sub_ann H as [HΔ [HΓ HΓ']]
+  end.
+
+#[local]
+Ltac gen_presup_anns :=
+  (on_all_hyp: fun H => gen_presup_ann H); invert_wf_gctx_ann; invert_wf_ctx_ann; clear_dups.
+
+
+(** * Soundness of annotated judgments *)
+Lemma soundness_gctx_lookup {P : PtsSig} : forall {Δ : gctx P} {annsΔ A so x},
+    {{ `#x : A @ so ∈ Δ @ annsΔ }} ->
+    {{ `#x : A ∈ Δ }}.
+Proof.
+  induction 1; mauto 2.
+Qed.
+
+#[local]
+Hint Resolve soundness_gctx_lookup : mcpts.
+
+Lemma soundness_ctx_lookup {P : PtsSig} : forall {Γ : ctx P} {annsΓ A so x},
+    {{ #x : A @ so ∈ Γ @ annsΓ }} ->
+    {{ #x : A ∈ Γ }}.
+Proof.
+  induction 1; mauto 2.
+Qed.
+
+#[local]
+Hint Resolve soundness_ctx_lookup : mcpts.
+
+Lemma soundness_ann_judg {P : PtsSig} :
+  (forall (Δ : gctx P) annsΔ, {{ ⊫ Δ @ annsΔ }} -> {{ ⊢ Δ }}) /\
+    (forall (Δ : gctx P) annsΔ Γ annsΓ, {{ Δ @ annsΔ ⊫ Γ @ annsΓ }} -> {{ Δ ⊢ Γ }}) /\
+    (forall (Δ : gctx P) annsΔ Γ annsΓ A so M, {{ Δ @ annsΔ ; Γ @ annsΓ ⊫ M : A @ so }} -> {{ Δ ; Γ ⊢ M : A }}) /\
+    (forall (Δ : gctx P) annsΔ Γ annsΓ A so, {{ Δ @ annsΔ ; Γ @ annsΓ ⊫ A @ so }} -> {{ Δ ; Γ ⊢ A }}) /\
+    (forall (Δ : gctx P) annsΔ Γ annsΓ Γ' annsΓ' σ, {{ Δ @ annsΔ ; Γ @ annsΓ ⊫s σ : Γ' @ annsΓ' }} -> {{ Δ ; Γ ⊢s σ : Γ' }}).
+Proof.
+  apply syntactic_wf_ann_mut_ind;
+    intros; mauto 2.
+  all: mauto 3.
+Qed.    
+
+#[local]
+Ltac solve_soundness_ann P :=
+  intros; pose proof @soundness_ann_judg P; destruct_conjs; eauto.
+
+Corollary soundness_wf_gctx {P : PtsSig} : forall {Δ : gctx P} {annsΔ},
+    {{ ⊫ Δ @ annsΔ }} ->
+    {{ ⊢ Δ }}.
+Proof. solve_soundness_ann P. Qed.
+
+Corollary soundness_wf_ctx {P : PtsSig} : forall {Δ : gctx P} {annsΔ Γ annsΓ},
+    {{ Δ @ annsΔ ⊫ Γ @ annsΓ}} ->
+    {{ Δ ⊢ Γ }}.
+Proof. solve_soundness_ann P. Qed.
+
+Corollary soundness_wf_exp {P : PtsSig} : forall {Δ : gctx P} {annsΔ Γ annsΓ A so M},
+    {{ Δ @ annsΔ ; Γ @ annsΓ ⊫ M : A @ so}} ->
+    {{ Δ ; Γ ⊢ M : A }}.
+Proof. solve_soundness_ann P. Qed.
+
+Corollary soundness_wf_typ {P : PtsSig} : forall {Δ : gctx P} {annsΔ Γ annsΓ A so},
+    {{ Δ @ annsΔ ; Γ @ annsΓ ⊫ A @ so}} ->
+    {{ Δ ; Γ ⊢ A }}.
+Proof. solve_soundness_ann P. Qed.
+
+Corollary soundness_wf_sub {P : PtsSig} : forall {Δ : gctx P} {annsΔ Γ annsΓ Γ' annsΓ' σ},
+    {{ Δ @ annsΔ ; Γ @ annsΓ ⊫s σ : Γ' @ annsΓ'}} ->
+    {{ Δ ; Γ ⊢s σ : Γ' }}.
+Proof. solve_soundness_ann P. Qed.
+
+#[export]
+Hint Resolve soundness_wf_gctx soundness_wf_ctx soundness_wf_exp soundness_wf_typ soundness_wf_sub : mcpts.
+ 
+
+(** * Completeness of annotated judgments *)
+Lemma complete_gctx_lookup {P : PtsSig} : forall {Δ : gctx P} {annsΔ A x},
+    {{ `#x : A ∈ Δ }} ->
+    {{ ⊫ Δ @ annsΔ }} ->
+    exists so, {{ `#x : A @ so ∈ Δ @ annsΔ }}.
+Proof.
+  intros * H.
+  gen annsΔ.
+  induction H; intros * HΔ;
+    dependent destruction HΔ; mauto 2.
+  specialize (IHgctx_lookup annsΔ0 ltac:(eassumption)) as [so'].
+  mauto 3.
+Qed.
+
+#[local]
+Hint Resolve complete_gctx_lookup : mcpts.
+
+Lemma complete_ctx_lookup {P : PtsSig} : forall {Δ : gctx P} {annsΔ Γ annsΓ A x},
+    {{ #x : A ∈ Γ }} ->
+    {{ Δ @ annsΔ ⊫ Γ @ annsΓ }} ->
+    exists so, {{ #x : A @ so ∈ Γ @ annsΓ }}.
+Proof.
+  intros * H.
+  gen annsΓ.
+  induction H; intros * HΓ;
+    dependent destruction HΓ; mauto 2.
+  specialize (IHctx_lookup annsΓ0 ltac:(eassumption)) as [so'].
+  mauto 3.
+Qed.
+
+#[local]
+Hint Resolve complete_ctx_lookup : mcpts.
+
+Lemma completeness_ann_judg {P : PtsSig} :
+  (forall (Δ : gctx P), {{ ⊢ Δ }} -> exists annsΔ, {{ ⊫ Δ @ annsΔ }}) /\
+    (forall (Δ : gctx P) Γ, {{ Δ ⊢ Γ }} -> exists annsΔ annsΓ, {{ Δ @ annsΔ ⊫ Γ @ annsΓ }}) /\
+    (forall (Δ : gctx P) Γ A M, {{ Δ ; Γ ⊢ M : A }} -> exists annsΔ annsΓ so, {{ Δ @ annsΔ ; Γ @ annsΓ ⊫ M : A @ so }}) /\
+    (forall (Δ : gctx P) Γ A, {{ Δ ; Γ ⊢ A }} -> exists annsΔ annsΓ so, {{ Δ @ annsΔ ; Γ @ annsΓ ⊫ A @ so }}) /\
+    (forall (Δ : gctx P) Γ Γ' σ, {{ Δ ; Γ ⊢s σ : Γ' }} -> exists annsΔ annsΓ annsΓ', {{ Δ @ annsΔ ; Γ @ annsΓ ⊫s σ : Γ' @ annsΓ' }}).
+Proof.
+  apply syntactic_wf_mut_ind';
+    intros; destruct_conjs; mauto 3;
+    gen_presup_anns;
+    try solve [repeat eexists; mauto 2].
+
+  - inversion HΓ; subst.
+    eexists; econstructor; mauto 3.
+
+  - 
+    
+#[local]
+Ltac gen_annotated_judg_IH P ann_gctx ann_ctx ann_exp ann_typ ann_sub :=
   match goal with 
   | H1 : {{ ⊢ ^?Γ }} |- _ => 
       let HΓ := fresh "HΓ" in
@@ -49,100 +356,8 @@ Ltac gen_sort_none P :=
     end;
   unmark_all.
 
-Lemma ctx_ann_decomp {P : PtsSig} : forall {Γ : ctx P} {A anns so}, {{ ⊫ Γ, A with so::anns }} -> {{ ⊫ Γ with anns }} /\ {{ Γ with anns ⊫ A @ so }}.
-Proof with now eauto.
-  inversion 1...
-Qed.
 
-#[local]
-Hint Resolve ctx_ann_decomp : mcpts.
 
-Corollary ctx_ann_decomp_left {P : PtsSig} : forall {Γ : ctx P} {A anns so}, {{ ⊫ Γ, A with so::anns }} -> {{ ⊫ Γ with anns }}.
-Proof with easy.
-  intros * ?%ctx_ann_decomp...
-Qed.
-
-Corollary ctx_ann_decomp_right {P : PtsSig} : forall {Γ : ctx P} {A anns so}, {{ ⊫ Γ, A with so::anns }} -> {{ Γ with anns ⊫ A @ so }}.
-Proof with easy.
-  intros * ?%ctx_ann_decomp...
-Qed.
-
-#[local]
-Hint Resolve ctx_ann_decomp_left ctx_ann_decomp_right : mcpts.
-
-Lemma presup_sub_ann_ctx_ann {P} : forall {Γ : ctx P} {anns anns' σ Δ},
-    {{ Γ with anns ⊫s σ : Δ with anns' }} -> {{ ⊫ Γ with anns }} /\ {{ ⊫ Δ with anns' }}.
-Proof.
-  induction 1; destruct_conjs; split; mauto 3.
-Qed.
-
-#[local]
-Hint Resolve presup_sub_ann_ctx_ann : mcpts.
-
-Lemma presup_sub_ann_ctx_ann_left {P} : forall {Γ : ctx P} {anns anns' σ Δ},
-    {{ Γ with anns ⊫s σ : Δ with anns' }} -> {{ ⊫ Γ with anns }}.
-Proof with easy.
-  intros * ?%presup_sub_ann_ctx_ann...
-Qed.
-
-Lemma presup_sub_ann_ctx_ann_right {P} : forall {Γ : ctx P} {anns anns' σ Δ},
-    {{ Γ with anns ⊫s σ : Δ with anns' }} -> {{ ⊫ Δ with anns' }}.
-Proof with easy.
-  intros * ?%presup_sub_ann_ctx_ann...
-Qed.
-
-#[local]
-Hint Resolve presup_sub_ann_ctx_ann_left presup_sub_ann_ctx_ann_right : mcpts.
-
-Lemma presup_exp_ann_ctx_ann {P} : forall {Γ : ctx P} {M A anns so},
-    {{ Γ with anns ⊫ M : A @ so }} -> {{ ⊫ Γ with anns }}.
-Proof.
-  induction 1; mauto 3.
-Qed.
-
-#[local]
-  Hint Resolve presup_exp_ann_ctx_ann : mcpts.
-
-Lemma presup_typ_ann_ctx_ann {P} : forall {Γ : ctx P} {A anns so},
-    {{ Γ with anns ⊫ A @ so }} -> {{ ⊫ Γ with anns }}.
-Proof.
-  induction 1; mauto 3.
-Qed.
-
-#[local]
-  Hint Resolve presup_typ_ann_ctx_ann : mcpts.
-
-Lemma ann_lookup_implies_lookup {P} : forall {anns : ctx_anns P} {so Γ x A},
-    {{ #x : A @ so ∈ Γ with anns }} ->
-    {{ ⊢ Γ }} ->
-    {{ #x : A ∈ Γ }}.
-Proof with mautosolve.
-  induction 1...
-Qed.  
-
-#[export]
-  Hint Resolve ann_lookup_implies_lookup : mcpts.
-
-Lemma lookup_implies_ann_lookup {P} : forall {anns : ctx_anns P} {Γ x A},
-    {{ #x : A ∈ Γ }} ->
-    {{ ⊫ Γ with anns }} ->
-    exists so, {{ #x : A @ so ∈ Γ with anns }}.
-Proof with mautosolve.
-  intros.
-  gen anns.
-  induction H.
-  - intros.
-    inversion H0; subst.
-    eexists.
-    mauto 2.
-  - intros.
-    inversion H0; subst.
-    assert (exists so : SortOption P, {{ # n : A @ so ∈ Γ with anns0 }}) as [] by mauto 2.
-    eexists; econstructor; mauto.
-Qed.
-
-#[export]
-  Hint Resolve lookup_implies_ann_lookup : mcpts.
 
 
 Lemma wf_ctx_implies_wf_ctx_ann {P} : forall {Γ : ctx P},
